Hashmap/DHashMap/Model.lean
@@ -1,0 +1,68 @@
+/-
+Copyright (c) 2024 Lean FRO, LLC. All rights reserved.
+Released under Apache 2.0 license as described in the file LICENSE.
+Authors: Markus Himmel
+-/
+import Hashmap.DHashMap.Basic
+
+/-!
+In this file we define functions for manipulating a hash map based on operations defined in terms of their buckets.
+Then we give "model implementations" of the hash map operations in terms of the basic building blocks and show that
+the actual operations are equal to the model implementations. This means that later we will be able to prove properties
+of the operations by proving general facts about the basic building blocks.
+-/
+
+set_option autoImplicit false
+
+universe u v
+
+variable {α : Type v} {β : α → Type v}
+
+namespace MyLean.DHashMap
+
+def bucket [Hashable α] (self : Array (AssocList α β)) (h : 0 < self.size) (k : α) : AssocList α β :=
+  let ⟨i, h⟩ := mkIdx (hash k) h
+  self[i]
+
+def updateBucket [Hashable α] (self : Array (AssocList α β)) (h : 0 < self.size) (k : α)
+    (f : AssocList α β → AssocList α β) : Array (AssocList α β) :=
+  let ⟨i, h⟩ := mkIdx (hash k) h
+  self.uset i (f self[i]) h
+
+@[simp]
+theorem size_updateBucket [Hashable α] {self : Array (AssocList α β)} {h : 0 < self.size} {k : α}
+    {f : AssocList α β → AssocList α β} : (updateBucket self h k f).size = self.size := by
+  simp [updateBucket]
+
+namespace Model
+
+def replace [BEq α] [Hashable α] (m : { m : Raw α β // 0 < m.buckets.size }) (a : α) (b : β a) : Raw α β :=
+  ⟨m.1.size, updateBucket m.1.buckets m.2 a (fun l => l.replace a b)⟩
+
+def cons [BEq α] [Hashable α] (m : { m : Raw α β // 0 < m.buckets.size }) (a : α) (b : β a) : { m : Raw α β // 0 < m.buckets.size } :=
+  ⟨⟨m.1.size + 1, updateBucket m.1.buckets m.2 a (fun l => l.cons a b)⟩, by simpa using m.2⟩
+
+def insert [BEq α] [Hashable α] (m : { m : Raw α β // 0 < m.buckets.size }) (a : α) (b : β a) : Raw α β :=
+  if (bucket m.1.buckets m.2 a).contains a then replace m a b else (Raw.expandIfNecessary (cons m a b)).1
+
+def findEntry? [BEq α] [Hashable α] (m : { m : Raw α β // 0 < m.buckets.size }) (a : α) : Option (Σ a, β a) :=
+  (bucket m.1.buckets m.2 a).findEntry? a
+
+end Model
+
+namespace Raw
+
+theorem insertWellFormed_eq_insertModel [BEq α] [Hashable α] (m : { m : Raw α β // 0 < m.buckets.size }) (a : α) (b : β a) :
+    (insertWellFormed m a b).1.1 = Model.insert m a b := by
+  rw [insertWellFormed, Model.insert, bucket]
+  dsimp
+  split
+  · rfl
+  · rfl
+
+theorem findEntry?WellFormed_eq [BEq α] [Hashable α] (m : { m : Raw α β // 0 < m.buckets.size }) (a : α) :
+    findEntry?WellFormed m a = Model.findEntry? m a := rfl
+
+end Raw
+
+end MyLean.DHashMap
